compiler/backend/backendScript.sml
@@ -256,7 +256,6 @@ val compile_eq_from_source = Q.store_thm("compile_eq_from_source",
   unabbrev_all_tac >>
   rpt (CHANGED_TAC (srw_tac[][] >> full_simp_tac(srw_ss())[] >> srw_tac[][] >> rev_full_simp_tac(srw_ss())[])));
 
-(*
 val to_livesets_def = Define`
   to_livesets (c:α backend$config) p =
   let (c',p) = to_data c p in
@@ -281,13 +280,14 @@ val from_livesets_def = Define`
   let (word_conf,asm_conf) = (c.word_to_word_conf,c.lab_conf.asm_conf) in
   let (n_oracles,col) = next_n_oracle (LENGTH p) word_conf.col_oracle in
   let alg = word_conf.reg_alg in
-  let prog_with_oracles = ZIP (n_oracles,ZIP(clashmovforec,p)) in
+  let prog_with_oracles = ZIP (n_oracles,ZIP(clashmovforce,p)) in
   let p =
-    MAP (λ(col_opt,((tree,moves,force),name_num,arg_count,prog)).
-      case oracle_colour_ok k col_opt tree prog of
+    MAP (λ(col_opt,((tree,moves,forced),name_num,arg_count,prog)).
+      case oracle_colour_ok k col_opt tree prog forced of
         NONE =>
           (let (clash_graph,_) = clash_tree_to_spg tree [] LN in
-             let col = reg_alloc alg clash_graph k moves
+           let ext_graph = FOLDR (λ(x,y) g. undir_g_insert x y g) clash_graph forced in
+             let col = reg_alloc alg ext_graph k moves
              in
                (name_num,arg_count,remove_must_terminate (apply_colour (total_colour col) prog)))
       | SOME col_prog => (name_num,arg_count,remove_must_terminate col_prog)) prog_with_oracles in
@@ -370,6 +370,5 @@ val to_data_change_config = Q.store_thm("to_data_change_config",
   rw[to_data_def,to_bvi_def,to_bvl_def,to_clos_def,to_pat_def,to_exh_def,to_dec_def,to_con_def,to_mod_def]
   \\ rpt (pairarg_tac \\ fs[]) \\ rw[] \\ fs[] \\ rfs[] \\ rveq \\ fs[] \\ rfs[] \\ rveq \\ fs[]
   \\ simp[config_component_equality]);
-*)
 
 val _ = export_theory();
